<?xml version="1.0"?>


<!DOCTYPE rdf:RDF [
    <!ENTITY terms "http://purl.org/dc/terms/" >
    <!ENTITY owl "http://www.w3.org/2002/07/owl#" >
    <!ENTITY dc "http://purl.org/dc/elements/1.1/" >
    <!ENTITY xsd "http://www.w3.org/2001/XMLSchema#" >
    <!ENTITY rdfs "http://www.w3.org/2000/01/rdf-schema#" >
    <!ENTITY rdf "http://www.w3.org/1999/02/22-rdf-syntax-ns#" >
]>


<rdf:RDF xmlns="http://envi.uef.fi/wavellite/wto#"
     xml:base="http://envi.uef.fi/wavellite/wto"
     xmlns:dc="http://purl.org/dc/elements/1.1/"
     xmlns:rdfs="http://www.w3.org/2000/01/rdf-schema#"
     xmlns:terms="http://purl.org/dc/terms/"
     xmlns:owl="http://www.w3.org/2002/07/owl#"
     xmlns:xsd="http://www.w3.org/2001/XMLSchema#"
     xmlns:rdf="http://www.w3.org/1999/02/22-rdf-syntax-ns#">
    <owl:Ontology rdf:about="http://envi.uef.fi/wavellite/wo/core">
        <terms:created rdf:datatype="&xsd;date">2014-01-01</terms:created>
        <terms:modified rdf:datatype="&xsd;date">2014-01-10</terms:modified>
        <dc:creator rdf:datatype="&xsd;string">Markus Stocker (University of Eastern Finland)</dc:creator>
        <dc:identifier rdf:datatype="&xsd;anyURI">http://envi.uef.fi/wavellite/wo/core</dc:identifier>
        <owl:versionInfo>1.0.0</owl:versionInfo>
        <rdfs:comment>The Wavellite task can be described as the acquisition and representation of situational knowledge from sensor data for environmental phenomena. The WTO describes the Wavellite entities that are relevant to this task.</rdfs:comment>
        <rdfs:seeAlso>http://www.uef.fi/en/envi/projects/wavellite</rdfs:seeAlso>
        <owl:imports rdf:resource="http://purl.oclc.org/NET/ssnx/ssn"/>
        <owl:imports rdf:resource="http://purl.org/linked-data/cube"/>
        <owl:imports rdf:resource="http://vistology.com/ont/2008/STO/STO.owl"/>
        <owl:imports rdf:resource="http://www.opengis.net/ont/geosparql"/>
        <owl:imports rdf:resource="http://www.w3.org/2006/time"/>
    </owl:Ontology>
    


    <!-- 
    ///////////////////////////////////////////////////////////////////////////////////////
    //
    // Annotation properties
    //
    ///////////////////////////////////////////////////////////////////////////////////////
     -->

    


    <!-- 
    ///////////////////////////////////////////////////////////////////////////////////////
    //
    // Datatypes
    //
    ///////////////////////////////////////////////////////////////////////////////////////
     -->

    


    <!-- 
    ///////////////////////////////////////////////////////////////////////////////////////
    //
    // Object Properties
    //
    ///////////////////////////////////////////////////////////////////////////////////////
     -->

    


    <!-- http://vistology.com/ont/2008/STO/STO.owl#hasAttribute -->

    <rdf:Description rdf:about="http://vistology.com/ont/2008/STO/STO.owl#hasAttribute">
        <rdfs:label xml:lang="en">has attribute</rdfs:label>
        <rdfs:isDefinedBy>http://vistology.com/ont/2008/STO/STO.owl</rdfs:isDefinedBy>
        <rdfs:subPropertyOf rdf:resource="http://www.loa-cnr.it/ontologies/DUL.owl#hasRegion"/>
    </rdf:Description>
    


    <!-- http://vistology.com/ont/2008/STO/STO.owl#hasAttributeValue -->

    <rdf:Description rdf:about="http://vistology.com/ont/2008/STO/STO.owl#hasAttributeValue">
        <rdfs:label xml:lang="en">has attribute value</rdfs:label>
        <rdfs:isDefinedBy>http://vistology.com/ont/2008/STO/STO.owl</rdfs:isDefinedBy>
        <rdfs:comment xml:lang="en">The STO object property relates a STO Attribute with a STO Value. Given that STO values are DUL Regions, we model this STO object property as a sub property of the DUL &apos;has region&apos;.</rdfs:comment>
        <rdfs:subPropertyOf rdf:resource="http://purl.oclc.org/NET/ssnx/ssn#hasValue"/>
    </rdf:Description>
    


    <!-- http://www.opengis.net/ont/geosparql#ehContains -->

    <rdf:Description rdf:about="http://www.opengis.net/ont/geosparql#ehContains">
        <rdfs:subPropertyOf rdf:resource="http://www.loa-cnr.it/ontologies/DUL.owl#hasPart"/>
    </rdf:Description>
    


    <!-- http://www.opengis.net/ont/geosparql#ehCoveredBy -->

    <rdf:Description rdf:about="http://www.opengis.net/ont/geosparql#ehCoveredBy">
        <rdfs:subPropertyOf rdf:resource="http://www.loa-cnr.it/ontologies/DUL.owl#isPartOf"/>
    </rdf:Description>
    


    <!-- http://www.opengis.net/ont/geosparql#ehCovers -->

    <rdf:Description rdf:about="http://www.opengis.net/ont/geosparql#ehCovers">
        <rdfs:subPropertyOf rdf:resource="http://www.loa-cnr.it/ontologies/DUL.owl#hasPart"/>
    </rdf:Description>
    


    <!-- http://www.opengis.net/ont/geosparql#ehEquals -->

    <rdf:Description rdf:about="http://www.opengis.net/ont/geosparql#ehEquals">
        <rdfs:subPropertyOf rdf:resource="http://www.loa-cnr.it/ontologies/DUL.owl#hasPart"/>
    </rdf:Description>
    


    <!-- http://www.opengis.net/ont/geosparql#ehInside -->

    <rdf:Description rdf:about="http://www.opengis.net/ont/geosparql#ehInside">
        <rdfs:subPropertyOf rdf:resource="http://www.loa-cnr.it/ontologies/DUL.owl#isPartOf"/>
    </rdf:Description>
    


    <!-- http://www.opengis.net/ont/geosparql#ehMeet -->

    <rdf:Description rdf:about="http://www.opengis.net/ont/geosparql#ehMeet">
        <rdfs:subPropertyOf rdf:resource="http://www.loa-cnr.it/ontologies/DUL.owl#hasCommonBoundary"/>
        <rdfs:subPropertyOf rdf:resource="http://www.loa-cnr.it/ontologies/DUL.owl#nearTo"/>
    </rdf:Description>
    


    <!-- http://www.opengis.net/ont/geosparql#ehOverlap -->

    <rdf:Description rdf:about="http://www.opengis.net/ont/geosparql#ehOverlap">
        <rdfs:subPropertyOf rdf:resource="http://www.loa-cnr.it/ontologies/DUL.owl#nearTo"/>
        <rdfs:subPropertyOf rdf:resource="http://www.loa-cnr.it/ontologies/DUL.owl#overlaps"/>
    </rdf:Description>
    


    <!-- http://www.opengis.net/ont/geosparql#hasGeometry -->

    <rdf:Description rdf:about="http://www.opengis.net/ont/geosparql#hasGeometry">
        <rdfs:subPropertyOf rdf:resource="http://www.loa-cnr.it/ontologies/DUL.owl#hasRegion"/>
    </rdf:Description>
    


    <!-- http://www.opengis.net/ont/geosparql#rcc8ec -->

    <rdf:Description rdf:about="http://www.opengis.net/ont/geosparql#rcc8ec">
        <rdfs:subPropertyOf rdf:resource="http://www.loa-cnr.it/ontologies/DUL.owl#hasCommonBoundary"/>
        <rdfs:subPropertyOf rdf:resource="http://www.loa-cnr.it/ontologies/DUL.owl#nearTo"/>
    </rdf:Description>
    


    <!-- http://www.opengis.net/ont/geosparql#rcc8eq -->

    <rdf:Description rdf:about="http://www.opengis.net/ont/geosparql#rcc8eq">
        <rdfs:subPropertyOf rdf:resource="http://www.loa-cnr.it/ontologies/DUL.owl#hasPart"/>
    </rdf:Description>
    


    <!-- http://www.opengis.net/ont/geosparql#rcc8ntpp -->

    <rdf:Description rdf:about="http://www.opengis.net/ont/geosparql#rcc8ntpp">
        <rdfs:subPropertyOf rdf:resource="http://www.loa-cnr.it/ontologies/DUL.owl#hasPart"/>
    </rdf:Description>
    


    <!-- http://www.opengis.net/ont/geosparql#rcc8ntppi -->

    <rdf:Description rdf:about="http://www.opengis.net/ont/geosparql#rcc8ntppi">
        <rdfs:subPropertyOf rdf:resource="http://www.loa-cnr.it/ontologies/DUL.owl#hasPart"/>
    </rdf:Description>
    


    <!-- http://www.opengis.net/ont/geosparql#rcc8po -->

    <rdf:Description rdf:about="http://www.opengis.net/ont/geosparql#rcc8po">
        <rdfs:subPropertyOf rdf:resource="http://www.loa-cnr.it/ontologies/DUL.owl#nearTo"/>
        <rdfs:subPropertyOf rdf:resource="http://www.loa-cnr.it/ontologies/DUL.owl#overlaps"/>
    </rdf:Description>
    


    <!-- http://www.opengis.net/ont/geosparql#rcc8tpp -->

    <rdf:Description rdf:about="http://www.opengis.net/ont/geosparql#rcc8tpp">
        <rdfs:subPropertyOf rdf:resource="http://www.loa-cnr.it/ontologies/DUL.owl#hasPart"/>
    </rdf:Description>
    


    <!-- http://www.opengis.net/ont/geosparql#rcc8tppi -->

    <rdf:Description rdf:about="http://www.opengis.net/ont/geosparql#rcc8tppi">
        <rdfs:subPropertyOf rdf:resource="http://www.loa-cnr.it/ontologies/DUL.owl#hasPart"/>
    </rdf:Description>
    


    <!-- http://www.opengis.net/ont/geosparql#sfContains -->

    <rdf:Description rdf:about="http://www.opengis.net/ont/geosparql#sfContains">
        <rdfs:subPropertyOf rdf:resource="http://www.loa-cnr.it/ontologies/DUL.owl#hasPart"/>
    </rdf:Description>
    


    <!-- http://www.opengis.net/ont/geosparql#sfCrosses -->

    <rdf:Description rdf:about="http://www.opengis.net/ont/geosparql#sfCrosses">
        <rdfs:subPropertyOf rdf:resource="http://www.loa-cnr.it/ontologies/DUL.owl#nearTo"/>
    </rdf:Description>
    


    <!-- http://www.opengis.net/ont/geosparql#sfEquals -->

    <rdf:Description rdf:about="http://www.opengis.net/ont/geosparql#sfEquals">
        <rdfs:subPropertyOf rdf:resource="http://www.loa-cnr.it/ontologies/DUL.owl#hasPart"/>
    </rdf:Description>
    


    <!-- http://www.opengis.net/ont/geosparql#sfIntersects -->

    <rdf:Description rdf:about="http://www.opengis.net/ont/geosparql#sfIntersects">
        <rdfs:subPropertyOf rdf:resource="http://www.loa-cnr.it/ontologies/DUL.owl#nearTo"/>
        <rdfs:subPropertyOf rdf:resource="http://www.loa-cnr.it/ontologies/DUL.owl#overlaps"/>
    </rdf:Description>
    


    <!-- http://www.opengis.net/ont/geosparql#sfOverlaps -->

    <rdf:Description rdf:about="http://www.opengis.net/ont/geosparql#sfOverlaps">
        <rdfs:subPropertyOf rdf:resource="http://www.loa-cnr.it/ontologies/DUL.owl#nearTo"/>
        <rdfs:subPropertyOf rdf:resource="http://www.loa-cnr.it/ontologies/DUL.owl#overlaps"/>
    </rdf:Description>
    


    <!-- http://www.opengis.net/ont/geosparql#sfTouches -->

    <rdf:Description rdf:about="http://www.opengis.net/ont/geosparql#sfTouches">
        <rdfs:subPropertyOf rdf:resource="http://www.loa-cnr.it/ontologies/DUL.owl#hasCommonBoundary"/>
        <rdfs:subPropertyOf rdf:resource="http://www.loa-cnr.it/ontologies/DUL.owl#nearTo"/>
    </rdf:Description>
    


    <!-- http://www.opengis.net/ont/geosparql#sfWithin -->

    <rdf:Description rdf:about="http://www.opengis.net/ont/geosparql#sfWithin">
        <rdfs:subPropertyOf rdf:resource="http://www.loa-cnr.it/ontologies/DUL.owl#isPartOf"/>
    </rdf:Description>
    


    <!-- http://www.w3.org/2004/02/skos/core#member -->

    <rdf:Description rdf:about="http://www.w3.org/2004/02/skos/core#member">
        <rdfs:subPropertyOf rdf:resource="http://www.loa-cnr.it/ontologies/DUL.owl#hasMember"/>
    </rdf:Description>
    


    <!-- http://www.w3.org/2006/time#after -->

    <rdf:Description rdf:about="http://www.w3.org/2006/time#after">
        <rdfs:label xml:lang="en">after</rdfs:label>
        <rdfs:isDefinedBy>http://www.w3.org/2006/time</rdfs:isDefinedBy>
        <rdfs:subPropertyOf rdf:resource="http://www.loa-cnr.it/ontologies/DUL.owl#follows"/>
        <rdfs:subPropertyOf rdf:resource="http://www.loa-cnr.it/ontologies/DUL.owl#hasRegion"/>
    </rdf:Description>
    


    <!-- http://www.w3.org/2006/time#before -->

    <rdf:Description rdf:about="http://www.w3.org/2006/time#before">
        <rdfs:label xml:lang="en">before</rdfs:label>
        <rdfs:isDefinedBy>http://www.w3.org/2006/time</rdfs:isDefinedBy>
        <rdfs:subPropertyOf rdf:resource="http://www.loa-cnr.it/ontologies/DUL.owl#hasRegion"/>
        <rdfs:subPropertyOf rdf:resource="http://www.loa-cnr.it/ontologies/DUL.owl#precedes"/>
    </rdf:Description>
    


    <!-- http://www.w3.org/2006/time#hasBeginning -->

    <rdf:Description rdf:about="http://www.w3.org/2006/time#hasBeginning">
        <rdfs:label xml:lang="en">has beginning</rdfs:label>
        <rdfs:isDefinedBy>http://www.w3.org/2006/time</rdfs:isDefinedBy>
        <rdfs:subPropertyOf rdf:resource="http://purl.oclc.org/NET/ssnx/ssn#startTime"/>
    </rdf:Description>
    


    <!-- http://www.w3.org/2006/time#hasDateTimeDescription -->

    <rdf:Description rdf:about="http://www.w3.org/2006/time#hasDateTimeDescription">
        <rdfs:label xml:lang="en">has dateTime description</rdfs:label>
        <rdfs:isDefinedBy>http://www.w3.org/2006/time</rdfs:isDefinedBy>
        <rdfs:subPropertyOf rdf:resource="http://www.loa-cnr.it/ontologies/DUL.owl#hasRegion"/>
    </rdf:Description>
    


    <!-- http://www.w3.org/2006/time#hasDurationDescription -->

    <rdf:Description rdf:about="http://www.w3.org/2006/time#hasDurationDescription">
        <rdfs:label xml:lang="en">has duration description</rdfs:label>
        <rdfs:isDefinedBy>http://www.w3.org/2006/time</rdfs:isDefinedBy>
        <rdfs:subPropertyOf rdf:resource="http://www.loa-cnr.it/ontologies/DUL.owl#hasRegion"/>
    </rdf:Description>
    


    <!-- http://www.w3.org/2006/time#hasEnd -->

    <rdf:Description rdf:about="http://www.w3.org/2006/time#hasEnd">
        <rdfs:label xml:lang="en">has end</rdfs:label>
        <rdfs:isDefinedBy>http://www.w3.org/2006/time</rdfs:isDefinedBy>
        <rdfs:subPropertyOf rdf:resource="http://purl.oclc.org/NET/ssnx/ssn#endTime"/>
    </rdf:Description>
    


    <!-- http://www.w3.org/2006/time#inDateTime -->

    <rdf:Description rdf:about="http://www.w3.org/2006/time#inDateTime">
        <rdfs:label xml:lang="en">in dateTime</rdfs:label>
        <rdfs:isDefinedBy>http://www.w3.org/2006/time</rdfs:isDefinedBy>
        <rdfs:subPropertyOf rdf:resource="http://www.loa-cnr.it/ontologies/DUL.owl#hasRegion"/>
    </rdf:Description>
    


    <!-- http://www.w3.org/2006/time#inside -->

    <rdf:Description rdf:about="http://www.w3.org/2006/time#inside">
        <rdfs:label xml:lang="en">inside</rdfs:label>
        <rdfs:isDefinedBy>http://www.w3.org/2006/time</rdfs:isDefinedBy>
        <rdfs:subPropertyOf rdf:resource="http://www.loa-cnr.it/ontologies/DUL.owl#hasRegion"/>
    </rdf:Description>
    


    <!-- http://www.w3.org/2006/time#intervalAfter -->

    <rdf:Description rdf:about="http://www.w3.org/2006/time#intervalAfter">
        <rdfs:label xml:lang="en">interval after</rdfs:label>
        <rdfs:isDefinedBy>http://www.w3.org/2006/time</rdfs:isDefinedBy>
        <rdfs:subPropertyOf rdf:resource="http://www.w3.org/2006/time#after"/>
    </rdf:Description>
    


    <!-- http://www.w3.org/2006/time#intervalContains -->

    <rdf:Description rdf:about="http://www.w3.org/2006/time#intervalContains">
        <rdfs:label xml:lang="en">interval contains</rdfs:label>
        <rdfs:isDefinedBy>http://www.w3.org/2006/time</rdfs:isDefinedBy>
        <rdfs:subPropertyOf rdf:resource="http://www.loa-cnr.it/ontologies/DUL.owl#hasPart"/>
        <rdfs:subPropertyOf rdf:resource="http://www.loa-cnr.it/ontologies/DUL.owl#hasRegion"/>
    </rdf:Description>
    


    <!-- http://www.w3.org/2006/time#intervalDuring -->

    <rdf:Description rdf:about="http://www.w3.org/2006/time#intervalDuring">
        <rdfs:label xml:lang="en">interval during</rdfs:label>
        <rdfs:isDefinedBy>http://www.w3.org/2006/time</rdfs:isDefinedBy>
        <rdfs:subPropertyOf rdf:resource="http://www.loa-cnr.it/ontologies/DUL.owl#hasRegion"/>
        <rdfs:subPropertyOf rdf:resource="http://www.loa-cnr.it/ontologies/DUL.owl#isPartOf"/>
    </rdf:Description>
    


    <!-- http://www.w3.org/2006/time#intervalEquals -->

    <rdf:Description rdf:about="http://www.w3.org/2006/time#intervalEquals">
        <rdfs:label xml:lang="en">interval equals</rdfs:label>
        <rdfs:isDefinedBy>http://www.w3.org/2006/time</rdfs:isDefinedBy>
        <rdfs:subPropertyOf rdf:resource="http://www.loa-cnr.it/ontologies/DUL.owl#hasPart"/>
        <rdfs:subPropertyOf rdf:resource="http://www.loa-cnr.it/ontologies/DUL.owl#hasRegion"/>
    </rdf:Description>
    


    <!-- http://www.w3.org/2006/time#intervalFinishedBy -->

    <rdf:Description rdf:about="http://www.w3.org/2006/time#intervalFinishedBy">
        <rdfs:label xml:lang="en">interval finished by</rdfs:label>
        <rdfs:isDefinedBy>http://www.w3.org/2006/time</rdfs:isDefinedBy>
        <rdfs:subPropertyOf rdf:resource="http://www.loa-cnr.it/ontologies/DUL.owl#hasRegion"/>
    </rdf:Description>
    


    <!-- http://www.w3.org/2006/time#intervalFinishes -->

    <rdf:Description rdf:about="http://www.w3.org/2006/time#intervalFinishes">
        <rdfs:label xml:lang="en">interval finishes</rdfs:label>
        <rdfs:isDefinedBy>http://www.w3.org/2006/time</rdfs:isDefinedBy>
        <rdfs:subPropertyOf rdf:resource="http://www.loa-cnr.it/ontologies/DUL.owl#hasRegion"/>
    </rdf:Description>
    


    <!-- http://www.w3.org/2006/time#intervalMeets -->

    <rdf:Description rdf:about="http://www.w3.org/2006/time#intervalMeets">
        <rdfs:label xml:lang="en">interval meets</rdfs:label>
        <rdfs:isDefinedBy>http://www.w3.org/2006/time</rdfs:isDefinedBy>
        <rdfs:subPropertyOf rdf:resource="http://www.loa-cnr.it/ontologies/DUL.owl#hasRegion"/>
        <rdfs:subPropertyOf rdf:resource="http://www.loa-cnr.it/ontologies/DUL.owl#nearTo"/>
    </rdf:Description>
    


    <!-- http://www.w3.org/2006/time#intervalMetBy -->

    <rdf:Description rdf:about="http://www.w3.org/2006/time#intervalMetBy">
        <rdfs:label xml:lang="en">interval met by</rdfs:label>
        <rdfs:isDefinedBy>http://www.w3.org/2006/time</rdfs:isDefinedBy>
        <rdfs:subPropertyOf rdf:resource="http://www.loa-cnr.it/ontologies/DUL.owl#hasRegion"/>
        <rdfs:subPropertyOf rdf:resource="http://www.loa-cnr.it/ontologies/DUL.owl#nearTo"/>
    </rdf:Description>
    


    <!-- http://www.w3.org/2006/time#intervalOverlappedBy -->

    <rdf:Description rdf:about="http://www.w3.org/2006/time#intervalOverlappedBy">
        <rdfs:label xml:lang="en">interval overlapped by</rdfs:label>
        <rdfs:isDefinedBy>http://www.w3.org/2006/time</rdfs:isDefinedBy>
        <rdfs:subPropertyOf rdf:resource="http://www.loa-cnr.it/ontologies/DUL.owl#hasRegion"/>
    </rdf:Description>
    


    <!-- http://www.w3.org/2006/time#intervalOverlaps -->

    <rdf:Description rdf:about="http://www.w3.org/2006/time#intervalOverlaps">
        <rdfs:label xml:lang="en">interval overlaps</rdfs:label>
        <rdfs:isDefinedBy>http://www.w3.org/2006/time</rdfs:isDefinedBy>
        <rdfs:subPropertyOf rdf:resource="http://www.loa-cnr.it/ontologies/DUL.owl#hasRegion"/>
        <rdfs:subPropertyOf rdf:resource="http://www.loa-cnr.it/ontologies/DUL.owl#overlaps"/>
    </rdf:Description>
    


    <!-- http://www.w3.org/2006/time#intervalStartedBy -->

    <rdf:Description rdf:about="http://www.w3.org/2006/time#intervalStartedBy">
        <rdfs:label xml:lang="en">interval started by</rdfs:label>
        <rdfs:isDefinedBy>http://www.w3.org/2006/time</rdfs:isDefinedBy>
        <rdfs:subPropertyOf rdf:resource="http://www.loa-cnr.it/ontologies/DUL.owl#hasRegion"/>
    </rdf:Description>
    


    <!-- http://www.w3.org/2006/time#intervalStarts -->

    <rdf:Description rdf:about="http://www.w3.org/2006/time#intervalStarts">
        <rdfs:label xml:lang="en">interval starts</rdfs:label>
        <rdfs:isDefinedBy>http://www.w3.org/2006/time</rdfs:isDefinedBy>
        <rdfs:subPropertyOf rdf:resource="http://www.loa-cnr.it/ontologies/DUL.owl#hasRegion"/>
    </rdf:Description>
    


    <!-- http://www.w3.org/2006/time#timeZone -->

    <rdf:Description rdf:about="http://www.w3.org/2006/time#timeZone">
        <rdfs:label xml:lang="en">time zone</rdfs:label>
        <rdfs:isDefinedBy>http://www.w3.org/2006/time</rdfs:isDefinedBy>
        <rdfs:subPropertyOf rdf:resource="http://www.loa-cnr.it/ontologies/DUL.owl#hasRegion"/>
    </rdf:Description>
    


    <!-- 
    ///////////////////////////////////////////////////////////////////////////////////////
    //
    // Data properties
    //
    ///////////////////////////////////////////////////////////////////////////////////////
     -->

    


    <!-- http://vistology.com/ont/2008/STO/STO.owl#attributeValue -->

    <rdf:Description rdf:about="http://vistology.com/ont/2008/STO/STO.owl#attributeValue">
        <rdfs:label xml:lang="en">The STO datatype property that relates a STO Value with an XSD datatype. Because STO Value is a DUL Region this property is a sub property of DUL &apos;has region data value&apos;.</rdfs:label>
        <rdfs:label xml:lang="en">attribute value</rdfs:label>
        <rdfs:isDefinedBy>http://vistology.com/ont/2008/STO/STO.owl</rdfs:isDefinedBy>
        <rdfs:subPropertyOf rdf:resource="http://www.loa-cnr.it/ontologies/DUL.owl#hasRegionDataValue"/>
    </rdf:Description>
    


    <!-- http://vistology.com/ont/2008/STO/STO.owl#certainty -->

    <rdf:Description rdf:about="http://vistology.com/ont/2008/STO/STO.owl#certainty">
        <rdfs:label xml:lang="en">certainty</rdfs:label>
        <rdfs:isDefinedBy>http://vistology.com/ont/2008/STO/STO.owl</rdfs:isDefinedBy>
        <rdfs:comment xml:lang="en">STO value is a DUL region. Thus, this datatype property is a sub property of DUL &apos;has region data value&apos;.</rdfs:comment>
        <rdfs:subPropertyOf rdf:resource="http://www.loa-cnr.it/ontologies/DUL.owl#hasRegionDataValue"/>
    </rdf:Description>
    


    <!-- http://www.opengis.net/ont/geosparql#coordinateDimension -->

    <rdf:Description rdf:about="http://www.opengis.net/ont/geosparql#coordinateDimension">
        <rdfs:subPropertyOf rdf:resource="http://www.loa-cnr.it/ontologies/DUL.owl#hasRegionDataValue"/>
    </rdf:Description>
    


    <!-- http://www.opengis.net/ont/geosparql#dimension -->

    <rdf:Description rdf:about="http://www.opengis.net/ont/geosparql#dimension">
        <rdfs:subPropertyOf rdf:resource="http://www.loa-cnr.it/ontologies/DUL.owl#hasRegionDataValue"/>
    </rdf:Description>
    


    <!-- http://www.opengis.net/ont/geosparql#isEmpty -->

    <rdf:Description rdf:about="http://www.opengis.net/ont/geosparql#isEmpty">
        <rdfs:subPropertyOf rdf:resource="http://www.loa-cnr.it/ontologies/DUL.owl#hasRegionDataValue"/>
    </rdf:Description>
    


    <!-- http://www.opengis.net/ont/geosparql#isSimple -->

    <rdf:Description rdf:about="http://www.opengis.net/ont/geosparql#isSimple">
        <rdfs:subPropertyOf rdf:resource="http://www.loa-cnr.it/ontologies/DUL.owl#hasRegionDataValue"/>
    </rdf:Description>
    


    <!-- http://www.opengis.net/ont/geosparql#spatialDimension -->

    <rdf:Description rdf:about="http://www.opengis.net/ont/geosparql#spatialDimension">
        <rdfs:subPropertyOf rdf:resource="http://www.loa-cnr.it/ontologies/DUL.owl#hasRegionDataValue"/>
    </rdf:Description>
    


    <!-- http://www.w3.org/2006/time#day -->

    <rdf:Description rdf:about="http://www.w3.org/2006/time#day">
        <rdfs:label xml:lang="en">day</rdfs:label>
        <rdfs:isDefinedBy>http://www.w3.org/2006/time</rdfs:isDefinedBy>
        <rdfs:subPropertyOf rdf:resource="http://www.loa-cnr.it/ontologies/DUL.owl#hasRegionDataValue"/>
    </rdf:Description>
    


    <!-- http://www.w3.org/2006/time#dayOfYear -->

    <rdf:Description rdf:about="http://www.w3.org/2006/time#dayOfYear">
        <rdfs:label xml:lang="en">day of year</rdfs:label>
        <rdfs:isDefinedBy>http://www.w3.org/2006/time</rdfs:isDefinedBy>
        <rdfs:subPropertyOf rdf:resource="http://www.loa-cnr.it/ontologies/DUL.owl#hasRegionDataValue"/>
    </rdf:Description>
    


    <!-- http://www.w3.org/2006/time#days -->

    <rdf:Description rdf:about="http://www.w3.org/2006/time#days">
        <rdfs:label xml:lang="en">days</rdfs:label>
        <rdfs:isDefinedBy>http://www.w3.org/2006/time</rdfs:isDefinedBy>
        <rdfs:subPropertyOf rdf:resource="http://www.loa-cnr.it/ontologies/DUL.owl#hasRegionDataValue"/>
    </rdf:Description>
    


    <!-- http://www.w3.org/2006/time#hour -->

    <rdf:Description rdf:about="http://www.w3.org/2006/time#hour">
        <rdfs:label xml:lang="en">hour</rdfs:label>
        <rdfs:isDefinedBy>http://www.w3.org/2006/time</rdfs:isDefinedBy>
        <rdfs:subPropertyOf rdf:resource="http://www.loa-cnr.it/ontologies/DUL.owl#hasRegionDataValue"/>
    </rdf:Description>
    


    <!-- http://www.w3.org/2006/time#hours -->

    <rdf:Description rdf:about="http://www.w3.org/2006/time#hours">
        <rdfs:label xml:lang="en">hours</rdfs:label>
        <rdfs:isDefinedBy>http://www.w3.org/2006/time</rdfs:isDefinedBy>
        <rdfs:subPropertyOf rdf:resource="http://www.loa-cnr.it/ontologies/DUL.owl#hasRegionDataValue"/>
    </rdf:Description>
    


    <!-- http://www.w3.org/2006/time#inXSDDateTime -->

    <rdf:Description rdf:about="http://www.w3.org/2006/time#inXSDDateTime">
        <rdfs:label xml:lang="en">in XSD dateTime</rdfs:label>
        <rdfs:isDefinedBy>http://www.w3.org/2006/time</rdfs:isDefinedBy>
        <rdfs:comment xml:lang="en">This OWL-Time datatype property relates an OWL-Time Instant to an XSD dateTime. Given that OWL-Time Instant is a DUL Region, this datatype property is modelled as a sub property of &apos;has region data value&apos;.</rdfs:comment>
        <rdfs:subPropertyOf rdf:resource="http://www.loa-cnr.it/ontologies/DUL.owl#hasRegionDataValue"/>
    </rdf:Description>
    


    <!-- http://www.w3.org/2006/time#minute -->

    <rdf:Description rdf:about="http://www.w3.org/2006/time#minute">
        <rdfs:label xml:lang="en">minute</rdfs:label>
        <rdfs:isDefinedBy>http://www.w3.org/2006/time</rdfs:isDefinedBy>
        <rdfs:subPropertyOf rdf:resource="http://www.loa-cnr.it/ontologies/DUL.owl#hasRegionDataValue"/>
    </rdf:Description>
    


    <!-- http://www.w3.org/2006/time#minutes -->

    <rdf:Description rdf:about="http://www.w3.org/2006/time#minutes">
        <rdfs:label xml:lang="en">minutes</rdfs:label>
        <rdfs:isDefinedBy>http://www.w3.org/2006/time</rdfs:isDefinedBy>
        <rdfs:subPropertyOf rdf:resource="http://www.loa-cnr.it/ontologies/DUL.owl#hasRegionDataValue"/>
    </rdf:Description>
    


    <!-- http://www.w3.org/2006/time#month -->

    <rdf:Description rdf:about="http://www.w3.org/2006/time#month">
        <rdfs:label xml:lang="en">month</rdfs:label>
        <rdfs:isDefinedBy>http://www.w3.org/2006/time</rdfs:isDefinedBy>
        <rdfs:subPropertyOf rdf:resource="http://www.loa-cnr.it/ontologies/DUL.owl#hasRegionDataValue"/>
    </rdf:Description>
    


    <!-- http://www.w3.org/2006/time#months -->

    <rdf:Description rdf:about="http://www.w3.org/2006/time#months">
        <rdfs:label xml:lang="en">months</rdfs:label>
        <rdfs:isDefinedBy>http://www.w3.org/2006/time</rdfs:isDefinedBy>
        <rdfs:subPropertyOf rdf:resource="http://www.loa-cnr.it/ontologies/DUL.owl#hasRegionDataValue"/>
    </rdf:Description>
    


    <!-- http://www.w3.org/2006/time#second -->

    <rdf:Description rdf:about="http://www.w3.org/2006/time#second">
        <rdfs:label xml:lang="en">second</rdfs:label>
        <rdfs:isDefinedBy>http://www.w3.org/2006/time</rdfs:isDefinedBy>
        <rdfs:subPropertyOf rdf:resource="http://www.loa-cnr.it/ontologies/DUL.owl#hasRegionDataValue"/>
    </rdf:Description>
    


    <!-- http://www.w3.org/2006/time#seconds -->

    <rdf:Description rdf:about="http://www.w3.org/2006/time#seconds">
        <rdfs:label xml:lang="en">seconds</rdfs:label>
        <rdfs:isDefinedBy>http://www.w3.org/2006/time</rdfs:isDefinedBy>
        <rdfs:subPropertyOf rdf:resource="http://www.loa-cnr.it/ontologies/DUL.owl#hasRegionDataValue"/>
    </rdf:Description>
    


    <!-- http://www.w3.org/2006/time#week -->

    <rdf:Description rdf:about="http://www.w3.org/2006/time#week">
        <rdfs:label xml:lang="en">week</rdfs:label>
        <rdfs:isDefinedBy>http://www.w3.org/2006/time</rdfs:isDefinedBy>
        <rdfs:subPropertyOf rdf:resource="http://www.loa-cnr.it/ontologies/DUL.owl#hasRegionDataValue"/>
    </rdf:Description>
    


    <!-- http://www.w3.org/2006/time#weeks -->

    <rdf:Description rdf:about="http://www.w3.org/2006/time#weeks">
        <rdfs:label xml:lang="en">weeks</rdfs:label>
        <rdfs:isDefinedBy>http://www.w3.org/2006/time</rdfs:isDefinedBy>
        <rdfs:subPropertyOf rdf:resource="http://www.loa-cnr.it/ontologies/DUL.owl#hasRegionDataValue"/>
    </rdf:Description>
    


    <!-- http://www.w3.org/2006/time#xsdDateTime -->

    <rdf:Description rdf:about="http://www.w3.org/2006/time#xsdDateTime">
        <rdfs:label xml:lang="en">XSD dateTime</rdfs:label>
        <rdfs:isDefinedBy>http://www.w3.org/2006/time</rdfs:isDefinedBy>
        <rdfs:subPropertyOf rdf:resource="http://www.loa-cnr.it/ontologies/DUL.owl#hasRegionDataValue"/>
    </rdf:Description>
    


    <!-- http://www.w3.org/2006/time#year -->

    <rdf:Description rdf:about="http://www.w3.org/2006/time#year">
        <rdfs:label xml:lang="en">year</rdfs:label>
        <rdfs:isDefinedBy>http://www.w3.org/2006/time</rdfs:isDefinedBy>
        <rdfs:subPropertyOf rdf:resource="http://www.loa-cnr.it/ontologies/DUL.owl#hasRegionDataValue"/>
    </rdf:Description>
    


    <!-- http://www.w3.org/2006/time#years -->

    <rdf:Description rdf:about="http://www.w3.org/2006/time#years">
        <rdfs:label xml:lang="en">years</rdfs:label>
        <rdfs:isDefinedBy>http://www.w3.org/2006/time</rdfs:isDefinedBy>
        <rdfs:subPropertyOf rdf:resource="http://www.loa-cnr.it/ontologies/DUL.owl#hasRegionDataValue"/>
    </rdf:Description>
    


    <!-- 
    ///////////////////////////////////////////////////////////////////////////////////////
    //
    // Classes
    //
    ///////////////////////////////////////////////////////////////////////////////////////
     -->

    


    <!-- http://purl.oclc.org/NET/ssnx/ssn#FeatureOfInterest -->

    <rdf:Description rdf:about="http://purl.oclc.org/NET/ssnx/ssn#FeatureOfInterest">
        <owl:equivalentClass rdf:resource="http://www.opengis.net/ont/geosparql#Feature"/>
    </rdf:Description>
    


    <!-- http://purl.oclc.org/NET/ssnx/ssn#Input -->

    <rdf:Description rdf:about="http://purl.oclc.org/NET/ssnx/ssn#Input">
        <rdfs:subClassOf rdf:resource="http://www.loa-cnr.it/ontologies/DUL.owl#InformationObject"/>
    </rdf:Description>
    


    <!-- http://purl.oclc.org/NET/ssnx/ssn#Output -->

    <rdf:Description rdf:about="http://purl.oclc.org/NET/ssnx/ssn#Output">
        <rdfs:subClassOf rdf:resource="http://www.loa-cnr.it/ontologies/DUL.owl#InformationObject"/>
    </rdf:Description>
    


    <!-- http://purl.org/NET/scovo#Dataset -->

    <rdf:Description rdf:about="http://purl.org/NET/scovo#Dataset">
        <rdfs:label xml:lang="en">Dataset</rdfs:label>
        <rdfs:subClassOf rdf:resource="http://www.loa-cnr.it/ontologies/DUL.owl#InformationObject"/>
        <rdfs:isDefinedBy>http://purl.org/NET/scovo</rdfs:isDefinedBy>
    </rdf:Description>
    


    <!-- http://purl.org/NET/scovo#Item -->

    <rdf:Description rdf:about="http://purl.org/NET/scovo#Item">
        <rdfs:label xml:lang="en">Item</rdfs:label>
        <rdfs:subClassOf rdf:resource="http://www.loa-cnr.it/ontologies/DUL.owl#InformationObject"/>
        <rdfs:isDefinedBy>http://purl.org/NET/scovo</rdfs:isDefinedBy>
    </rdf:Description>
    


    <!-- http://purl.org/linked-data/cube#Attachable -->

    <rdf:Description rdf:about="http://purl.org/linked-data/cube#Attachable">
        <rdfs:subClassOf rdf:resource="http://www.loa-cnr.it/ontologies/DUL.owl#InformationObject"/>
        <rdfs:comment xml:lang="en">We model datasets, observations of datasets, and slices as DUL information objects.</rdfs:comment>
    </rdf:Description>
    


    <!-- http://purl.org/linked-data/cube#CodeList -->

    <rdf:Description rdf:about="http://purl.org/linked-data/cube#CodeList">
        <rdfs:label xml:lang="en">Code list</rdfs:label>
        <rdfs:subClassOf rdf:resource="http://www.loa-cnr.it/ontologies/DUL.owl#Collection"/>
        <rdfs:isDefinedBy>http://purl.org/linked-data/cube</rdfs:isDefinedBy>
        <rdfs:comment xml:lang="en">A QB code list is a DUL collection, specifically a collection of codes.</rdfs:comment>
    </rdf:Description>
    


    <!-- http://purl.org/linked-data/cube#ComponentProperty -->

    <rdf:Description rdf:about="http://purl.org/linked-data/cube#ComponentProperty">
        <rdfs:subClassOf rdf:resource="http://www.loa-cnr.it/ontologies/DUL.owl#SocialObjectAttribute"/>
        <rdfs:comment xml:lang="en">QB component properties are considered to be &apos;statistical attributes over a collection of entities&apos; and, thus, DUL social attributes.</rdfs:comment>
    </rdf:Description>
    


    <!-- http://purl.org/linked-data/cube#ComponentSet -->

    <rdf:Description rdf:about="http://purl.org/linked-data/cube#ComponentSet">
        <rdfs:subClassOf rdf:resource="http://www.loa-cnr.it/ontologies/DUL.owl#InformationObject"/>
    </rdf:Description>
    


    <!-- http://purl.org/linked-data/cube#ObservationGroup -->

    <rdf:Description rdf:about="http://purl.org/linked-data/cube#ObservationGroup">
        <rdfs:subClassOf rdf:resource="http://www.loa-cnr.it/ontologies/DUL.owl#InformationObject"/>
    </rdf:Description>
    


    <!-- http://vistology.com/ont/2008/STO/STO.owl#Agent -->

    <rdf:Description rdf:about="http://vistology.com/ont/2008/STO/STO.owl#Agent">
        <rdfs:label xml:lang="en">Agent</rdfs:label>
        <owl:equivalentClass rdf:resource="http://www.loa-cnr.it/ontologies/DUL.owl#Agent"/>
        <rdfs:isDefinedBy>http://vistology.com/ont/2008/STO/STO.owl</rdfs:isDefinedBy>
    </rdf:Description>
    


    <!-- http://vistology.com/ont/2008/STO/STO.owl#Attribute -->

    <rdf:Description rdf:about="http://vistology.com/ont/2008/STO/STO.owl#Attribute">
        <rdfs:label xml:lang="en">Attribute</rdfs:label>
        <rdfs:subClassOf rdf:resource="http://www.loa-cnr.it/ontologies/DUL.owl#Region"/>
        <rdfs:subClassOf>
            <owl:Class>
                <owl:unionOf rdf:parseType="Collection">
                    <rdf:Description rdf:about="http://www.loa-cnr.it/ontologies/DUL.owl#PhysicalAttribute"/>
                    <rdf:Description rdf:about="http://www.loa-cnr.it/ontologies/DUL.owl#SocialObjectAttribute"/>
                </owl:unionOf>
            </owl:Class>
        </rdfs:subClassOf>
        <rdfs:isDefinedBy>http://vistology.com/ont/2008/STO/STO.owl</rdfs:isDefinedBy>
        <rdfs:comment xml:lang="en">STO Attribute is modelled as a Region and may be a DUL physical attribute or a DUL social attribute.</rdfs:comment>
    </rdf:Description>
    


    <!-- http://vistology.com/ont/2008/STO/STO.owl#Dimensionality -->

    <rdf:Description rdf:about="http://vistology.com/ont/2008/STO/STO.owl#Dimensionality">
        <rdfs:label xml:lang="en">Dimensionality</rdfs:label>
        <rdfs:subClassOf rdf:resource="http://www.loa-cnr.it/ontologies/DUL.owl#UnitOfMeasure"/>
        <rdfs:comment xml:lang="en">A STO Dimensionality has members meter, meter per second, second. Hence, we model it as a DUL &apos;unit of measure&apos;.</rdfs:comment>
        <rdfs:isDefinedBy>http://vistology.com/ont/2008/STO/STO.owl</rdfs:isDefinedBy>
    </rdf:Description>
    


    <!-- http://vistology.com/ont/2008/STO/STO.owl#ElementaryInfon -->

    <rdf:Description rdf:about="http://vistology.com/ont/2008/STO/STO.owl#ElementaryInfon">
        <rdfs:label xml:lang="en">Elementary infon</rdfs:label>
        <rdfs:subClassOf rdf:resource="http://www.loa-cnr.it/ontologies/DUL.owl#InformationObject"/>
        <rdfs:comment xml:lang="en">A STO ElementaryInfon is modelled as a DUL information object. According to the Situation Theory, an elementary infon is a tuple consisting of a relation, relevant objects, and a polarity. </rdfs:comment>
        <rdfs:isDefinedBy>http://vistology.com/ont/2008/STO/STO.owl</rdfs:isDefinedBy>
    </rdf:Description>
    


    <!-- http://vistology.com/ont/2008/STO/STO.owl#Event -->

    <rdf:Description rdf:about="http://vistology.com/ont/2008/STO/STO.owl#Event">
        <rdfs:label xml:lang="en">Event</rdfs:label>
        <rdfs:isDefinedBy>http://vistology.com/ont/2008/STO/STO.owl</rdfs:isDefinedBy>
    </rdf:Description>
    


    <!-- http://vistology.com/ont/2008/STO/STO.owl#Individual -->

    <rdf:Description rdf:about="http://vistology.com/ont/2008/STO/STO.owl#Individual">
        <rdfs:label xml:lang="en">Individual</rdfs:label>
        <rdfs:subClassOf rdf:resource="http://www.loa-cnr.it/ontologies/DUL.owl#Object"/>
        <rdfs:subClassOf>
            <owl:Class>
                <owl:unionOf rdf:parseType="Collection">
                    <rdf:Description rdf:about="http://www.loa-cnr.it/ontologies/DUL.owl#PhysicalObject"/>
                    <rdf:Description rdf:about="http://www.loa-cnr.it/ontologies/DUL.owl#SocialObject"/>
                </owl:unionOf>
            </owl:Class>
        </rdfs:subClassOf>
        <rdfs:comment xml:lang="en">A STO Individual may be a DUL physical object or a DUL social object.</rdfs:comment>
        <rdfs:isDefinedBy>http://vistology.com/ont/2008/STO/STO.owl</rdfs:isDefinedBy>
    </rdf:Description>
    


    <!-- http://vistology.com/ont/2008/STO/STO.owl#Location -->

    <rdf:Description rdf:about="http://vistology.com/ont/2008/STO/STO.owl#Location">
        <rdfs:label xml:lang="en">Location</rdfs:label>
        <rdfs:subClassOf rdf:resource="http://www.loa-cnr.it/ontologies/DUL.owl#PhysicalAttribute"/>
        <rdfs:comment xml:lang="en">STO location is a DUL physical attribute because location is a physical value of a physical object.</rdfs:comment>
        <rdfs:isDefinedBy xml:lang="en">http://vistology.com/ont/2008/STO/STO.owl</rdfs:isDefinedBy>
    </rdf:Description>
    


    <!-- http://vistology.com/ont/2008/STO/STO.owl#Object -->

    <rdf:Description rdf:about="http://vistology.com/ont/2008/STO/STO.owl#Object">
        <rdfs:label xml:lang="en">Object</rdfs:label>
        <rdfs:subClassOf rdf:resource="http://www.loa-cnr.it/ontologies/DUL.owl#Entity"/>
        <rdfs:subClassOf>
            <owl:Class>
                <owl:unionOf rdf:parseType="Collection">
                    <rdf:Description rdf:about="http://vistology.com/ont/2008/STO/STO.owl#Event"/>
                    <rdf:Description rdf:about="http://www.loa-cnr.it/ontologies/DUL.owl#Abstract"/>
                    <rdf:Description rdf:about="http://www.loa-cnr.it/ontologies/DUL.owl#Object"/>
                </owl:unionOf>
            </owl:Class>
        </rdfs:subClassOf>
        <rdfs:comment xml:lang="en">A STO object can be a DUL object, a DUL abstract, or a DUL event. These classes are disjoint; hence, the chosen modelling. A STO object may be a DUL event because a STO individual may be a DUL event.</rdfs:comment>
        <rdfs:isDefinedBy>http://vistology.com/ont/2008/STO/STO.owl</rdfs:isDefinedBy>
    </rdf:Description>
    


    <!-- http://vistology.com/ont/2008/STO/STO.owl#Proposition -->

    <rdf:Description rdf:about="http://vistology.com/ont/2008/STO/STO.owl#Proposition">
        <rdfs:label xml:lang="en">Proposition</rdfs:label>
        <rdfs:subClassOf rdf:resource="http://www.loa-cnr.it/ontologies/DUL.owl#Description"/>
        <rdfs:comment xml:lang="en">STO propositions are modelled as DUL social objects, specifically as DUL descriptions.</rdfs:comment>
        <rdfs:isDefinedBy>http://vistology.com/ont/2008/STO/STO.owl</rdfs:isDefinedBy>
    </rdf:Description>
    


    <!-- http://vistology.com/ont/2008/STO/STO.owl#Relation -->

    <rdf:Description rdf:about="http://vistology.com/ont/2008/STO/STO.owl#Relation">
        <rdfs:label xml:lang="en">Relation</rdfs:label>
        <rdfs:subClassOf rdf:resource="http://www.loa-cnr.it/ontologies/DUL.owl#FormalEntity"/>
        <rdfs:comment xml:lang="en">A STO relation is modelled as an DUL abstract entity, as a relation (e.g. velocity) is not located in time-space. Specifically, we model STO relations as DUL formal entities.</rdfs:comment>
        <rdfs:isDefinedBy>http://vistology.com/ont/2008/STO/STO.owl</rdfs:isDefinedBy>
        <rdfs:seeAlso>http://www.loa-cnr.it/ontologies/DUL.owl#Relation</rdfs:seeAlso>
    </rdf:Description>
    


    <!-- http://vistology.com/ont/2008/STO/STO.owl#Rule -->

    <rdf:Description rdf:about="http://vistology.com/ont/2008/STO/STO.owl#Rule">
        <rdfs:label xml:lang="en">Rule</rdfs:label>
        <rdfs:subClassOf rdf:resource="http://www.loa-cnr.it/ontologies/DUL.owl#FormalEntity"/>
        <rdfs:comment xml:lang="en">A STO rule is modelled as a DUL abstract entity, as it is not located in time-space. Specifically, rules are DUL formal entities.</rdfs:comment>
        <rdfs:isDefinedBy>http://vistology.com/ont/2008/STO/STO.owl</rdfs:isDefinedBy>
    </rdf:Description>
    


    <!-- http://vistology.com/ont/2008/STO/STO.owl#Situation -->

    <rdf:Description rdf:about="http://vistology.com/ont/2008/STO/STO.owl#Situation">
        <rdfs:label xml:lang="en">Situation</rdfs:label>
        <rdfs:subClassOf rdf:resource="http://www.loa-cnr.it/ontologies/DUL.owl#Situation"/>
        <rdfs:isDefinedBy>http://vistology.com/ont/2008/STO/STO.owl</rdfs:isDefinedBy>
    </rdf:Description>
    


    <!-- http://vistology.com/ont/2008/STO/STO.owl#Value -->

    <rdf:Description rdf:about="http://vistology.com/ont/2008/STO/STO.owl#Value">
        <rdfs:label xml:lang="en">Value</rdfs:label>
        <rdfs:subClassOf rdf:resource="http://www.loa-cnr.it/ontologies/DUL.owl#Region"/>
        <rdfs:comment xml:lang="en">A STO Value relates via datatype property attributeValue to the actual value. Thus, a STO Value is modelled as a DUL Region.</rdfs:comment>
        <rdfs:isDefinedBy>http://vistology.com/ont/2008/STO/STO.owl</rdfs:isDefinedBy>
    </rdf:Description>
    


    <!-- http://vistology.com/ont/2008/STO/STO.owl#Velocity -->

    <rdf:Description rdf:about="http://vistology.com/ont/2008/STO/STO.owl#Velocity">
        <rdfs:label xml:lang="en">Velocity</rdfs:label>
        <rdfs:subClassOf rdf:resource="http://www.loa-cnr.it/ontologies/DUL.owl#PhysicalAttribute"/>
        <rdfs:comment xml:lang="en">STO velocity is a DUL physical attribute, because velocity is a physical value of a physical object.</rdfs:comment>
        <rdfs:isDefinedBy>http://vistology.com/ont/2008/STO/STO.owl</rdfs:isDefinedBy>
    </rdf:Description>
    


    <!-- http://www.loa-cnr.it/ontologies/DUL.owl#Agent -->

    <rdf:Description rdf:about="http://www.loa-cnr.it/ontologies/DUL.owl#Agent"/>
    


    <!-- http://www.loa-cnr.it/ontologies/DUL.owl#Concept -->

    <rdf:Description rdf:about="http://www.loa-cnr.it/ontologies/DUL.owl#Concept">
        <owl:equivalentClass rdf:resource="http://www.w3.org/2004/02/skos/core#Concept"/>
    </rdf:Description>
    


    <!-- http://www.opengis.net/ont/geosparql#Feature -->

    <rdf:Description rdf:about="http://www.opengis.net/ont/geosparql#Feature">
        <rdfs:comment xml:lang="en">A GeoSPARQL feature is equivalent to SSN &apos;feature of interest&apos;. Feature may be a DUL event or a DUL object, specifically it may be a DUL physical object (e.g. a DUL natural person) or a DUL social object (e.g. a DUL place).</rdfs:comment>
    </rdf:Description>
    


    <!-- http://www.opengis.net/ont/geosparql#Geometry -->

    <rdf:Description rdf:about="http://www.opengis.net/ont/geosparql#Geometry">
        <rdfs:subClassOf rdf:resource="http://www.loa-cnr.it/ontologies/DUL.owl#SpaceRegion"/>
    </rdf:Description>
    


    <!-- http://www.opengis.net/ont/geosparql#SpatialObject -->

    <rdf:Description rdf:about="http://www.opengis.net/ont/geosparql#SpatialObject">
        <rdfs:subClassOf rdf:resource="http://www.loa-cnr.it/ontologies/DUL.owl#Entity"/>
        <rdfs:subClassOf>
            <owl:Class>
                <owl:unionOf rdf:parseType="Collection">
                    <rdf:Description rdf:about="http://vistology.com/ont/2008/STO/STO.owl#Event"/>
                    <rdf:Description rdf:about="http://www.loa-cnr.it/ontologies/DUL.owl#Abstract"/>
                    <rdf:Description rdf:about="http://www.loa-cnr.it/ontologies/DUL.owl#Object"/>
                </owl:unionOf>
            </owl:Class>
        </rdfs:subClassOf>
        <rdfs:comment xml:lang="en">GeoSPARQL spatial objects are modelled as DUL entities. They subsume both features and geometries. Features are real world phenomena, e.g. as in SSN &apos;feature of interest&apos;. The SSN feature of interest is modelled as being either a DUL event or a DUL object, which are disjoint. Thus, a GeoSPARQL spatial object is necessarily subsumbed by both DUL event and DUL object, too. In addition, GeoSPARQL geometries are DUL abstract entities, specifically DUL space regions. Hence, a GeoSPARQL spatial object is also subsumed by DUL abstract.</rdfs:comment>
    </rdf:Description>
    


    <!-- http://www.w3.org/2004/02/skos/core#Collection -->

    <rdf:Description rdf:about="http://www.w3.org/2004/02/skos/core#Collection">
        <rdfs:subClassOf rdf:resource="http://www.loa-cnr.it/ontologies/DUL.owl#Collection"/>
        <rdfs:comment xml:lang="en">SKOS collections are specifically collections of concepts. We thus model SKOS collections as DUL collections, hence social objects.</rdfs:comment>
    </rdf:Description>
    


    <!-- http://www.w3.org/2004/02/skos/core#Concept -->

    <rdf:Description rdf:about="http://www.w3.org/2004/02/skos/core#Concept">
        <rdfs:subClassOf rdf:resource="http://www.loa-cnr.it/ontologies/DUL.owl#SocialObject"/>
    </rdf:Description>
    


    <!-- http://www.w3.org/2004/02/skos/core#ConceptScheme -->

    <rdf:Description rdf:about="http://www.w3.org/2004/02/skos/core#ConceptScheme">
        <rdfs:subClassOf rdf:resource="http://www.loa-cnr.it/ontologies/DUL.owl#SocialObject"/>
    </rdf:Description>
    


    <!-- http://www.w3.org/2006/time#DateTimeDescription -->

    <rdf:Description rdf:about="http://www.w3.org/2006/time#DateTimeDescription">
        <rdfs:label xml:lang="en">Date time description</rdfs:label>
        <rdfs:subClassOf rdf:resource="http://www.loa-cnr.it/ontologies/DUL.owl#TimeInterval"/>
        <rdfs:isDefinedBy>http://www.w3.org/2006/time</rdfs:isDefinedBy>
        <rdfs:comment xml:lang="en">A OWL-Time date time description relates to a OWL-Time instant via the OWL-Time &apos;has date time description&apos; object property. Given that OWL-Time instant is a region and that the corresponding date time description is an alternative way to represent the instant we model OWL-Time date time descriptions also as DUL regions.</rdfs:comment>
    </rdf:Description>
    


    <!-- http://www.w3.org/2006/time#DayOfWeek -->

    <rdf:Description rdf:about="http://www.w3.org/2006/time#DayOfWeek">
        <rdfs:label xml:lang="en">Day of week</rdfs:label>
        <rdfs:subClassOf rdf:resource="http://www.loa-cnr.it/ontologies/DUL.owl#UnitOfMeasure"/>
        <rdfs:isDefinedBy>http://www.w3.org/2006/time</rdfs:isDefinedBy>
        <rdfs:seeAlso>http://en.wikipedia.org/wiki/Day</rdfs:seeAlso>
        <rdfs:comment xml:lang="en">The OWL-Time days of a week (meaning individuals for each of the seven days of a week) are modelled as DUL concepts, specifically DUL units of measure. A OWL-Time day of a week is a day and a day is a unit of time. Days of a week are related to OWL-Time date time descriptions (DUL regions) via the OWL-Time &apos;day of week&apos; object property.</rdfs:comment>
    </rdf:Description>
    


    <!-- http://www.w3.org/2006/time#DurationDescription -->

    <rdf:Description rdf:about="http://www.w3.org/2006/time#DurationDescription">
        <rdfs:label xml:lang="en">Duration description</rdfs:label>
        <rdfs:subClassOf rdf:resource="http://www.loa-cnr.it/ontologies/DUL.owl#TimeInterval"/>
        <rdfs:isDefinedBy>http://www.w3.org/2006/time</rdfs:isDefinedBy>
        <rdfs:comment xml:lang="en">A OWL-Time duration description relates to a OWL-Time date time interval via the OWL-Time &apos;has duration description&apos; object property. Given that OWL-Time date time interval is a region and that the corresponding duration description is a representation of the elapsed time between the two instants defining the interval we model OWL-Time duration descriptions also as DUL regions.</rdfs:comment>
    </rdf:Description>
    


    <!-- http://www.w3.org/2006/time#TemporalEntity -->

    <rdf:Description rdf:about="http://www.w3.org/2006/time#TemporalEntity">
        <rdfs:label xml:lang="en">Temporal entity</rdfs:label>
        <rdfs:subClassOf rdf:resource="http://www.loa-cnr.it/ontologies/DUL.owl#TimeInterval"/>
        <rdfs:comment xml:lang="en">OWL-Time temporal enties are modelled as DUL time intervals, as we consider both time instants and time intervals to be DUL time intervals, meaning that a OWL-Time instant is a DUL time interval with coinciding start and end time.</rdfs:comment>
        <rdfs:isDefinedBy>http://www.w3.org/2006/time</rdfs:isDefinedBy>
    </rdf:Description>
    


    <!-- http://www.w3.org/2006/time#TemporalUnit -->

    <rdf:Description rdf:about="http://www.w3.org/2006/time#TemporalUnit">
        <rdfs:label xml:lang="en">Temporal unit</rdfs:label>
        <rdfs:subClassOf rdf:resource="http://www.loa-cnr.it/ontologies/DUL.owl#UnitOfMeasure"/>
        <rdfs:isDefinedBy>http://www.w3.org/2006/time</rdfs:isDefinedBy>
    </rdf:Description>
    


    <!-- http://www.w3.org/2006/timezone#TimeZone -->

    <rdf:Description rdf:about="http://www.w3.org/2006/timezone#TimeZone">
        <rdfs:label xml:lang="en">Time zone</rdfs:label>
        <rdfs:subClassOf rdf:resource="http://www.loa-cnr.it/ontologies/DUL.owl#Region"/>
        <rdfs:seeAlso>http://en.wikipedia.org/wiki/Time_zone</rdfs:seeAlso>
        <rdfs:comment xml:lang="en">A time zone is a region that has a uniform standard time for legal, commercial, and social purposes. It is convenient for areas in close commercial or other communication to keep the same time, so time zones tend to follow the boundaries of countries and their subdivisions.</rdfs:comment>
    </rdf:Description>
    


    <!-- 
    ///////////////////////////////////////////////////////////////////////////////////////
    //
    // Annotations
    //
    ///////////////////////////////////////////////////////////////////////////////////////
     -->

    <rdf:Description rdf:about="http://vistology.com/ont/2008/STO/STO.owl#focalRelation">
        <rdfs:label xml:lang="en">focal relation</rdfs:label>
        <rdfs:isDefinedBy>http://vistology.com/ont/2008/STO/STO.owl</rdfs:isDefinedBy>
    </rdf:Description>
    <rdf:Description rdf:about="http://vistology.com/ont/2008/STO/STO.owl#anchor2Inverse">
        <rdfs:label xml:lang="en">anchor2 inverse</rdfs:label>
        <rdfs:isDefinedBy>http://vistology.com/ont/2008/STO/STO.owl</rdfs:isDefinedBy>
    </rdf:Description>
    <rdf:Description rdf:about="http://vistology.com/ont/2008/STO/STO.owl#impliedByRule">
        <rdfs:label xml:lang="en">implied by rule</rdfs:label>
        <rdfs:isDefinedBy>http://vistology.com/ont/2008/STO/STO.owl</rdfs:isDefinedBy>
    </rdf:Description>
    <rdf:Description rdf:about="http://vistology.com/ont/2008/STO/STO.owl#relevantRelation">
        <rdfs:label xml:lang="en">relevant relation</rdfs:label>
        <rdfs:isDefinedBy>http://vistology.com/ont/2008/STO/STO.owl</rdfs:isDefinedBy>
    </rdf:Description>
    <rdf:Description rdf:about="http://vistology.com/ont/2008/STO/STO.owl#par3Type">
        <rdfs:label xml:lang="en">par3 type</rdfs:label>
        <rdfs:isDefinedBy>http://vistology.com/ont/2008/STO/STO.owl</rdfs:isDefinedBy>
    </rdf:Description>
    <rdf:Description rdf:about="http://www.w3.org/2006/time#dayOfWeek">
        <rdfs:label xml:lang="en">day of week</rdfs:label>
        <rdfs:isDefinedBy>http://www.w3.org/2006/time</rdfs:isDefinedBy>
    </rdf:Description>
    <rdf:Description rdf:about="http://www.w3.org/2006/time#unitType">
        <rdfs:label xml:lang="en">unit type</rdfs:label>
        <rdfs:isDefinedBy>http://www.w3.org/2006/time</rdfs:isDefinedBy>
    </rdf:Description>
    <rdf:Description rdf:about="http://www.w3.org/2006/time#Instant">
        <rdfs:label xml:lang="en">Instant</rdfs:label>
        <rdfs:isDefinedBy>http://www.w3.org/2006/time</rdfs:isDefinedBy>
    </rdf:Description>
    <rdf:Description rdf:about="http://vistology.com/ont/2008/STO/STO.owl#supportedBySituation">
        <rdfs:label xml:lang="en">supperted by situation</rdfs:label>
        <rdfs:isDefinedBy>http://vistology.com/ont/2008/STO/STO.owl</rdfs:isDefinedBy>
    </rdf:Description>
    <rdf:Description rdf:about="http://www.w3.org/2006/time#ProperInterval">
        <rdfs:label xml:lang="en">Propert interval</rdfs:label>
        <rdfs:isDefinedBy>http://www.w3.org/2006/time</rdfs:isDefinedBy>
    </rdf:Description>
    <rdf:Description rdf:about="http://vistology.com/ont/2008/STO/STO.owl#anchor3Inverse">
        <rdfs:label xml:lang="en">anchor3 inverse</rdfs:label>
        <rdfs:isDefinedBy>http://vistology.com/ont/2008/STO/STO.owl</rdfs:isDefinedBy>
    </rdf:Description>
    <rdf:Description rdf:about="http://vistology.com/ont/2008/STO/STO.owl#utterance">
        <rdfs:label xml:lang="en">utterance</rdfs:label>
        <rdfs:isDefinedBy>http://vistology.com/ont/2008/STO/STO.owl</rdfs:isDefinedBy>
    </rdf:Description>
    <rdf:Description rdf:about="http://vistology.com/ont/2008/STO/STO.owl#referringSituation">
        <rdfs:label xml:lang="en">referring situation</rdfs:label>
        <rdfs:isDefinedBy>http://vistology.com/ont/2008/STO/STO.owl</rdfs:isDefinedBy>
    </rdf:Description>
    <rdf:Description rdf:about="http://vistology.com/ont/2008/STO/STO.owl#Utterance">
        <rdfs:label xml:lang="en">Utterance</rdfs:label>
        <rdfs:isDefinedBy>http://vistology.com/ont/2008/STO/STO.owl</rdfs:isDefinedBy>
    </rdf:Description>
    <rdf:Description rdf:about="http://vistology.com/ont/2008/STO/STO.owl#polarity">
        <rdfs:label xml:lang="en">polarity</rdfs:label>
        <rdfs:isDefinedBy>http://vistology.com/ont/2008/STO/STO.owl</rdfs:isDefinedBy>
    </rdf:Description>
    <rdf:Description rdf:about="http://vistology.com/ont/2008/STO/STO.owl#FocalSituation">
        <rdfs:label xml:lang="en">Focal situation</rdfs:label>
        <rdfs:isDefinedBy>http://vistology.com/ont/2008/STO/STO.owl</rdfs:isDefinedBy>
    </rdf:Description>
    <rdf:Description rdf:about="http://vistology.com/ont/2008/STO/STO.owl#TYP">
        <rdfs:label xml:lang="en">TYP</rdfs:label>
        <rdfs:isDefinedBy>http://vistology.com/ont/2008/STO/STO.owl</rdfs:isDefinedBy>
    </rdf:Description>
    <rdf:Description rdf:about="http://vistology.com/ont/2008/STO/STO.owl#resourceSituation">
        <rdfs:label xml:lang="en">resource situation</rdfs:label>
        <rdfs:isDefinedBy>http://vistology.com/ont/2008/STO/STO.owl</rdfs:isDefinedBy>
    </rdf:Description>
    <rdf:Description rdf:about="http://www.w3.org/2006/time#Year">
        <rdfs:label xml:lang="en">Year</rdfs:label>
        <rdfs:isDefinedBy>http://www.w3.org/2006/time</rdfs:isDefinedBy>
    </rdf:Description>
    <rdf:Description rdf:about="http://vistology.com/ont/2008/STO/STO.owl#anchor1">
        <rdfs:label xml:lang="en">anchor1</rdfs:label>
        <rdfs:isDefinedBy>http://vistology.com/ont/2008/STO/STO.owl</rdfs:isDefinedBy>
    </rdf:Description>
    <rdf:Description rdf:about="http://www.w3.org/2006/time#Interval">
        <rdfs:label xml:lang="en">Interval</rdfs:label>
        <rdfs:isDefinedBy>http://www.w3.org/2006/time</rdfs:isDefinedBy>
    </rdf:Description>
    <rdf:Description rdf:about="http://vistology.com/ont/2008/STO/STO.owl#relation">
        <rdfs:label xml:lang="en">relation</rdfs:label>
        <rdfs:isDefinedBy>http://vistology.com/ont/2008/STO/STO.owl</rdfs:isDefinedBy>
    </rdf:Description>
    <rdf:Description rdf:about="http://vistology.com/ont/2008/STO/STO.owl#anchor2">
        <rdfs:label xml:lang="en">anchor2</rdfs:label>
        <rdfs:isDefinedBy>http://vistology.com/ont/2008/STO/STO.owl</rdfs:isDefinedBy>
    </rdf:Description>
    <rdf:Description rdf:about="http://vistology.com/ont/2008/STO/STO.owl#anchor3">
        <rdfs:label xml:lang="en">anchor3</rdfs:label>
        <rdfs:isDefinedBy>http://vistology.com/ont/2008/STO/STO.owl</rdfs:isDefinedBy>
    </rdf:Description>
    <rdf:Description rdf:about="http://www.w3.org/2006/time#intervalBefore">
        <rdfs:label xml:lang="en">interval before</rdfs:label>
        <rdfs:isDefinedBy>http://www.w3.org/2006/time</rdfs:isDefinedBy>
    </rdf:Description>
    <rdf:Description rdf:about="http://vistology.com/ont/2008/STO/STO.owl#utteredBy">
        <rdfs:label xml:lang="en">uttered by</rdfs:label>
        <rdfs:isDefinedBy>http://vistology.com/ont/2008/STO/STO.owl</rdfs:isDefinedBy>
    </rdf:Description>
    <rdf:Description rdf:about="http://vistology.com/ont/2008/STO/STO.owl#UtteranceSituation">
        <rdfs:label xml:lang="en">Utterance situation</rdfs:label>
        <rdfs:isDefinedBy>http://vistology.com/ont/2008/STO/STO.owl</rdfs:isDefinedBy>
    </rdf:Description>
    <rdf:Description rdf:about="http://vistology.com/ont/2008/STO/STO.owl#focalIndividual">
        <rdfs:label xml:lang="en">focal individual</rdfs:label>
        <rdfs:isDefinedBy>http://vistology.com/ont/2008/STO/STO.owl</rdfs:isDefinedBy>
    </rdf:Description>
    <rdf:Description rdf:about="http://vistology.com/ont/2008/STO/STO.owl#supportedInfon">
        <rdfs:label xml:lang="en">supported infon</rdfs:label>
        <rdfs:isDefinedBy>http://vistology.com/ont/2008/STO/STO.owl</rdfs:isDefinedBy>
    </rdf:Description>
    <rdf:Description rdf:about="http://www.w3.org/2006/time#DateTimeInterval">
        <rdfs:label xml:lang="en">DateTime interval</rdfs:label>
        <rdfs:isDefinedBy>http://www.w3.org/2006/time</rdfs:isDefinedBy>
    </rdf:Description>
    <rdf:Description rdf:about="http://vistology.com/ont/2008/STO/STO.owl#relevantSituation">
        <rdfs:label xml:lang="en">relevant situation</rdfs:label>
        <rdfs:isDefinedBy>http://vistology.com/ont/2008/STO/STO.owl</rdfs:isDefinedBy>
    </rdf:Description>
    <rdf:Description rdf:about="http://vistology.com/ont/2008/STO/STO.owl#query">
        <rdfs:label xml:lang="en">query</rdfs:label>
        <rdfs:isDefinedBy>http://vistology.com/ont/2008/STO/STO.owl</rdfs:isDefinedBy>
    </rdf:Description>
    <rdf:Description rdf:about="http://vistology.com/ont/2008/STO/STO.owl#utteranceSituation">
        <rdfs:label xml:lang="en">utterance situation</rdfs:label>
        <rdfs:isDefinedBy>http://vistology.com/ont/2008/STO/STO.owl</rdfs:isDefinedBy>
    </rdf:Description>
    <rdf:Description rdf:about="http://vistology.com/ont/2008/STO/STO.owl#focalSituation">
        <rdfs:label xml:lang="en">focal situation</rdfs:label>
        <rdfs:isDefinedBy>http://vistology.com/ont/2008/STO/STO.owl</rdfs:isDefinedBy>
    </rdf:Description>
    <rdf:Description rdf:about="http://vistology.com/ont/2008/STO/STO.owl#anchor1Inverse">
        <rdfs:label xml:lang="en">anchor1 inverse</rdfs:label>
        <rdfs:isDefinedBy>http://vistology.com/ont/2008/STO/STO.owl</rdfs:isDefinedBy>
    </rdf:Description>
    <rdf:Description rdf:about="http://vistology.com/ont/2008/STO/STO.owl#Time">
        <rdfs:label xml:lang="en">Time</rdfs:label>
        <rdfs:comment xml:lang="en">STO time is an attribute of an object in an infon, i.e. STO individuals. A STO individual may be a DUL physical object, a DUL social object, or a DUL event. Thus, STO time cannot be specialized as a DUL social attribute.</rdfs:comment>
        <rdfs:isDefinedBy>http://vistology.com/ont/2008/STO/STO.owl</rdfs:isDefinedBy>
    </rdf:Description>
    <rdf:Description rdf:about="http://vistology.com/ont/2008/STO/STO.owl#par2Type">
        <rdfs:label xml:lang="en">par2 type</rdfs:label>
        <rdfs:isDefinedBy>http://vistology.com/ont/2008/STO/STO.owl</rdfs:isDefinedBy>
    </rdf:Description>
    <rdf:Description rdf:about="http://vistology.com/ont/2008/STO/STO.owl#dimensionality">
        <rdfs:label xml:lang="en">dimensionality</rdfs:label>
        <rdfs:isDefinedBy>http://vistology.com/ont/2008/STO/STO.owl</rdfs:isDefinedBy>
    </rdf:Description>
    <rdf:Description rdf:about="http://vistology.com/ont/2008/STO/STO.owl#par1Type">
        <rdfs:label xml:lang="en">par1 type</rdfs:label>
        <rdfs:isDefinedBy>http://vistology.com/ont/2008/STO/STO.owl</rdfs:isDefinedBy>
    </rdf:Description>
    <rdf:Description rdf:about="http://vistology.com/ont/2008/STO/STO.owl#Polarity">
        <rdfs:label xml:lang="en">Polarity</rdfs:label>
        <rdfs:isDefinedBy>http://vistology.com/ont/2008/STO/STO.owl</rdfs:isDefinedBy>
    </rdf:Description>
    <rdf:Description rdf:about="http://vistology.com/ont/2008/STO/STO.owl#involves">
        <rdfs:label xml:lang="en">involves</rdfs:label>
        <rdfs:isDefinedBy>http://vistology.com/ont/2008/STO/STO.owl</rdfs:isDefinedBy>
    </rdf:Description>
    <rdf:Description rdf:about="http://vistology.com/ont/2008/STO/STO.owl#relevantIndividual">
        <rdfs:label xml:lang="en">relevant individual</rdfs:label>
        <rdfs:isDefinedBy>http://vistology.com/ont/2008/STO/STO.owl</rdfs:isDefinedBy>
    </rdf:Description>
    <rdf:Description rdf:about="http://www.w3.org/2006/time#January">
        <rdfs:label xml:lang="en">January</rdfs:label>
        <rdfs:isDefinedBy>http://www.w3.org/2006/time</rdfs:isDefinedBy>
    </rdf:Description>
    <rdf:Description rdf:about="http://vistology.com/ont/2008/STO/STO.owl#PropertyRelation">
        <rdfs:label xml:lang="en">PropertyRelation</rdfs:label>
        <rdfs:isDefinedBy>http://vistology.com/ont/2008/STO/STO.owl</rdfs:isDefinedBy>
    </rdf:Description>
    <rdf:Description rdf:about="http://vistology.com/ont/2008/STO/STO.owl#ResourceSituation">
        <rdfs:label xml:lang="en">Resource situation</rdfs:label>
        <rdfs:isDefinedBy>http://vistology.com/ont/2008/STO/STO.owl</rdfs:isDefinedBy>
    </rdf:Description>
    <rdf:Description rdf:about="http://vistology.com/ont/2008/STO/STO.owl#Sentence">
        <rdfs:label xml:lang="en">Sentence</rdfs:label>
        <rdfs:comment xml:lang="en">STO sentence may be an attribute of both a DUL physical object or a DUL social object.</rdfs:comment>
        <rdfs:isDefinedBy>http://vistology.com/ont/2008/STO/STO.owl</rdfs:isDefinedBy>
    </rdf:Description>
    <rdf:Description rdf:about="http://vistology.com/ont/2008/STO/STO.owl#RelevantIndividual">
        <rdfs:label xml:lang="en">Relevant individual</rdfs:label>
        <rdfs:isDefinedBy>http://vistology.com/ont/2008/STO/STO.owl</rdfs:isDefinedBy>
    </rdf:Description>
</rdf:RDF>



<!-- Generated by the OWL API (version 3.3.1957) http://owlapi.sourceforge.net -->

